Snap

IIO.fst
@@ -1,13 +1,13 @@
-module M4wp
+module IIO
 
 open Common
 open IOStHist
 
-let m4wp_invariant_pre (pi_check : monitorable_prop) (s0:events_trace) : Type0 =
+let iio_invariant_pre (pi_check : monitorable_prop) (s0:events_trace) : Type0 =
   enforced_globally default_check s0 &&
   enforced_globally pi_check s0
 
-let m4wp_invariant_post
+let iio_invariant_post
   (#a:Type)
   (pi_check : monitorable_prop)
   (s0:events_trace)
@@ -20,10 +20,10 @@ let m4wp_invariant_post
   | Inl v -> let (s1, r) = v in s1 == (apply_changes s0 local_trace)
   | Inr _ -> True)
 
-effect M4wp
+effect IIO
   (a:Type)
   (pi_check : monitorable_prop) 
   (post : events_trace -> maybe (events_trace * a) -> events_trace -> Type0) =
   IOStHist a
-    (requires (m4wp_invariant_pre pi_check))
-    (ensures (fun h r le -> m4wp_invariant_post pi_check h r le /\ post h r le))
+    (requires (iio_invariant_pre pi_check))
+    (ensures (fun h r le -> iio_invariant_post pi_check h r le /\ post h r le))
