IO.fst
@@ -1,0 +1,167 @@
+module IO
+
+open FStar.Tactics
+open ExtraTactics
+
+open Common
+open IIO.Free
+
+let iohist_post a = maybe a -> events_trace -> Type0  // local_events (from old to new)
+let iohist_wpty a = events_trace -> iohist_post a -> Type0  // past_events (from new to old; reversed compared with local_events)
+
+unfold
+let iohist_return_wp (a:Type) (x:a) : iohist_wpty a =
+  fun past_events p -> p (Inl x) []
+
+unfold
+let compute_post (a b:Type) (past_events:events_trace) (kw : a -> iohist_wpty b) (p:iohist_post b)
+  : iohist_post a =
+      (fun result local_events -> 
+        match result with
+        | Inl result -> (
+            kw result
+            ((List.rev local_events) @ past_events) 
+            (fun result' local_events' -> 
+                p result' (local_events @ local_events')))
+        | Inr err -> p (Inr err) local_events)
+
+unfold
+let iohist_bind_wp (a:Type) (b:Type) (w : iohist_wpty a) (kw : a -> iohist_wpty b) : iohist_wpty b =
+  fun past_events p -> 
+    w past_events (compute_post a b past_events kw p)
+
+unfold let gen_post #a (post:iohist_post a) (event:io_event) = 
+  fun x local_events -> post x (event :: local_events)
+
+unfold let convert_call_to_event (cmd:io_cmds) (args:args cmd) (res:resm cmd) =
+  match cmd with
+  | Openfile -> EOpenfile args res
+  | Read -> ERead args res
+  | Close -> EClose args res
+
+let rec iohist_interpretation #a
+  (m : io a) 
+  (p : iohist_post a) : Type0 = 
+  match m with
+  | Return x -> p (Inl x) []
+  | Throw err -> p (Inr err) []
+  | Cont (Call cmd args fnc) -> (
+    forall res. (
+      FStar.WellFounded.axiom1 fnc res;
+      let event : io_event = convert_call_to_event cmd args res in
+      iohist_interpretation (fnc res) (gen_post p event)))
+
+
+// REFINED COMPUTATION MONAD (repr)
+let irepr (a:Type) (wp:iohist_wpty a) =
+  h:events_trace -> post:iohist_post a ->
+    Pure (io a)
+      (requires (wp h post))
+      (ensures (fun (t:io a) -> iohist_interpretation t post))
+
+let ireturn (a : Type) (x : a) : irepr a (iohist_return_wp a x) =
+  fun _ _ -> io_return a x
+
+let w = iohist_wpty
+
+unfold
+val w_ord (#a : Type) : w a -> w a -> Type0
+let w_ord wp1 wp2 = forall h p. wp1 h p ==> wp2 h p
+
+unfold
+let apply_changes (old_state local_trace:events_trace) = (List.rev local_trace) @ old_state
+
+
+let ibind (a b : Type) (wp_v : w a) (wp_f: a -> w b) (v : irepr a wp_v)
+  (f : (x:a -> irepr b (wp_f x))) : irepr b (iohist_bind_wp _ _ wp_v wp_f) =
+  fun h p -> 
+    let t = (io_bind a b 
+        (v h (compute_post a b h wp_f p))
+        (fun x ->
+          assume (wp_f x h p);
+           f x h p)) in
+    assume (iohist_interpretation t p);
+    t
+
+unfold
+let isubcomp (a:Type) (wp1 wp2: w a) (f : irepr a wp1) :
+  Pure (irepr a wp2) (requires w_ord wp2 wp1) (ensures fun _ -> True) = f
+
+unfold
+let wp_if_then_else (#a:Type) (wp1 wp2:w a) (b:bool) : w a =
+  fun h p -> (b ==> wp1 h p) /\ ((~b) ==> wp2 h p)
+
+unfold
+let i_if_then_else (a : Type) (wp1 wp2 : w a) (f : irepr a wp1) (g : irepr a wp2) (b : bool) : Type =
+  irepr a (wp_if_then_else wp1 wp2 b)
+
+total
+reifiable
+reflectable
+layered_effect {
+  IOwp : a:Type -> wp : iohist_wpty a -> Effect
+  with
+       repr       = irepr
+     ; return     = ireturn
+     ; bind       = ibind
+
+     ; subcomp      = isubcomp
+     ; if_then_else = i_if_then_else
+}
+
+let lift_pure_iowp (a:Type) (wp:pure_wp a) (f:(eqtype_as_type unit -> PURE a wp)) :
+  Pure (irepr a (fun s0 p -> wp (fun r -> p (Inl r) []))) (requires True)
+                    (ensures (fun _ -> True))
+  = fun s0 p -> let r = elim_pure f (fun r -> p (Inl r) []) in io_return _ r
+
+sub_effect PURE ~> IOwp = lift_pure_iowp
+  
+effect IO
+  (a:Type)
+  (pre : events_trace -> Type0)
+  (post : events_trace -> maybe a -> events_trace -> Type0) =
+  IOwp a (fun (h:events_trace) (p:iohist_post a) ->
+    pre h /\ (forall res le. post h res le ==>  p res le))
+
+let rec is_open (fd:file_descr) (past_events: events_trace) :
+  Tot bool =
+  match past_events with
+  | [] -> false
+  | h :: tail -> match h with
+               | EOpenfile _ (Inl fd') ->
+                   if fd = fd' then true
+                   else is_open fd tail
+               | EClose fd' _ -> 
+                    if fd = fd' then false
+                    else is_open fd tail
+               | _ -> is_open fd tail
+
+val default_check : monitorable_prop
+let default_check (state:events_trace) (action:action_type) =
+  match action with
+  | (| Openfile, fnm |) -> true
+  | (| Read, fd |) -> is_open fd state
+  | (| Close, fd |) -> is_open fd state
+
+
+let static_cmd
+  (cmd : io_cmds)
+  (argz : io_args cmd) :
+  IO (res cmd)
+    (requires (fun h -> default_check h (| cmd, argz |)))
+    (ensures (fun h r local_trace ->
+      local_trace == [convert_call_to_event cmd argz r]
+      /\ enforced_locally default_check h local_trace
+  )) =
+  IOwp?.reflect(fun _ _ -> io_all cmd argz)
+
+let openfile = static_cmd Openfile
+let read = static_cmd Read
+let close = static_cmd Close
+
+let testStat2 () : 
+  IO unit (fun h -> True) (fun h _ le -> enforced_locally default_check h le) =
+  let fd = openfile "../Makefile" in
+  let msg = read fd in
+  close fd;
+  ()
